src/Bedrock/Field/Synthesis/Examples/riscv_with_c/wrapper_template.s
@@ -1,3 +1,0 @@
-.section .text
-.globl _start
-_start: .incbin "FILENAME"
