src/Bedrock/Field/Synthesis/Examples/riscv_with_c/poly1305_compile.v
@@ -72,7 +72,9 @@ Definition allFuns: list Syntax.func := [
   UnsaturatedSolinas.from_bytes
 ].
 
-Definition e := map.of_list allFuns.
+Notation src_env := (SortedListString.map (list string * list string * Syntax.cmd.cmd)).
+
+Definition e: src_env := map.of_list allFuns.
 
 (* stack grows from high addreses to low addresses, first stack word will be written to
    (stack_pastend-8), next stack word to (stack_pastend-16) etc *)
@@ -89,14 +91,73 @@ Definition ml: MemoryLayout := {|
 
 Unset Printing Coercions. (* https://github.com/mit-plv/fiat-crypto/issues/899 *)
 
-(*
-Definition asm: list Instruction.
-  (*Time*) (let r := eval vm_compute in (compile ml e) in
-            match r with
-            | Some (?x, _) => exact x
-            end). (* 2.328 secs *)
-Defined.
-*)
+Definition compiled := Eval vm_compute in (compile ml e).
+
+Definition asm: list Instruction :=
+  match compiled with
+  | Some (l, _) => l
+  | None => []
+  end.
+
+Notation MapStrZ := (SortedListString.map Z).
+
+Definition positions: MapStrZ :=
+  match compiled with
+  | Some (_, e) => e
+  | None => map.empty
+  end.
+
+Definition LF : string := String (Coq.Strings.Ascii.Ascii false true false true false false false false) "".
+
+Definition ZToStr(z: Z): string := DecimalString.NilZero.string_of_int (BinInt.Z.to_int z).
+Definition natToStr(n: nat): string := ZToStr (Z.of_nat n).
+
+Fixpoint save_arg_regs(n: nat): string :=
+  match n with
+  | O => ""
+  | S m => save_arg_regs m ++ "  sw sp, a" ++ natToStr m ++ ", (" ++ ZToStr (-4 * Z.of_nat n) ++ ")" ++ LF
+  end.
+
+Fixpoint load_res_regs(n: nat)(offset: Z): string :=
+  match n with
+  | O => ""
+  | S m => load_res_regs m offset ++
+           "  lw a" ++ natToStr m ++ ", sp, (" ++ ZToStr (offset + -4 * Z.of_nat n) ++ ")" ++ LF
+  end.
+
+Definition call(mypos: Z)(e_src: src_env)(e_pos: MapStrZ)(f: string): (string * Z) :=
+  match map.get e_src f, map.get e_pos f with
+  | Some (argvars, resvars, body), Some funpos => (
+  "  addi sp, sp, (-4)" ++ LF ++
+  "  sw sp, ra, (0)" ++ LF ++
+  save_arg_regs (List.length argvars) ++
+  "  jalr ra, (" ++ ZToStr (funpos - (mypos + 4 * (2 + Z.of_nat (List.length argvars)))) ++ ")" ++ LF ++
+  load_res_regs (List.length resvars) (- Z.of_nat (List.length argvars)) ++
+  "  lw ra, sp, (0)" ++ LF ++
+  "  addi sp, sp, (4)" ++ LF ++
+  "  ret" ++ LF,
+  4 * (Z.of_nat (2 + List.length argvars + 1 + List.length resvars + 3)))
+  | _, _ => ("ERROR: " ++ f ++ " not found", -1)
+  end.
+
+Fixpoint wrappers(mypos: Z)(e_src: src_env)(e_pos: MapStrZ)(fs: list string): string :=
+  match fs with
+  | f :: rest => let '(s, l) := call mypos e_src e_pos f in
+                 f ++ ":" ++ LF ++ s ++ wrappers (mypos + l) e_src e_pos rest
+  | nil => ""
+  end.
+
+Definition asm_str: string :=
+  Eval vm_compute in
+  ".section .text" ++ LF ++
+  "bedrock2functions: .incbin ""tmp.bin""" ++ LF ++
+  wrappers (4 * (Z.of_nat (List.length asm))) e positions (map.keys positions).
+
+From bedrock2 Require Import ToCString Bytedump.
+Local Open Scope bytedump_scope.
+Goal True.
+  let c_code := eval vm_compute in (byte_list_of_string asm_str) in idtac c_code.
+Abort.
 
 Definition valid_instructions: list Instruction -> Prop :=
   Forall (fun i : Instruction => verify i RV32IM).
@@ -119,12 +180,10 @@ Proof.
   all: fail.
 *)
 
-(*
 Module PrintAssembly.
   Import riscv.Utility.InstructionNotations.
   Goal True. let r := eval unfold asm in asm in idtac (* r *). Abort.
 End PrintAssembly.
-*)
 
 Require Import Crypto.Bedrock.Field.Synthesis.Examples.riscv.SyscallNumbers.
 Import RegisterNames Decode.
@@ -282,7 +341,7 @@ https://www.devever.net/~hl/incbin
 (* Note: this must be Coq.Init.Byte.byte, not coqutil.Byte.byte,
    which is a Notation for `(Coq.Init.Byte.byte: Type)` and doesn't
    work with bedrock2.Hexdump. *)
-Definition as_bytes: list Coq.Init.Byte.byte := instrencode probe_mem.
+Definition as_bytes: list Coq.Init.Byte.byte := instrencode asm.
 
 Module PrintBytes.
   Import bedrock2.Hexdump.
