src/Bedrock/Field/Synthesis/Examples/riscv_with_c/poly1305_wrap.v
@@ -1,0 +1,165 @@
+(* Before opening this file in PG, run `RISCV_COMPILATION=1 make bedrock2-backend` in
+   the fiat-crypto root directory, which will build all dependencies, including
+   bedrock2, riscv-coq, the bedrock2 compiler, and all the required fiat-crypto files,
+   and make sure to accept the COQPATH updates in .dir-locals.el *)
+
+Set Warnings "-notation-incompatible-format".
+
+Require Import Crypto.Bedrock.Field.Synthesis.Examples.X1305_32.
+
+Require Import Coq.Lists.List.
+Import ListNotations.
+Require Import compiler.Pipeline.
+Require Import riscv.Spec.Decode.
+Require Import riscv.Utility.Words32Naive.
+Require Import riscv.Utility.DefaultMemImpl32.
+Require Import riscv.Utility.Monads.
+Require Import compiler.util.Common.
+Require Import coqutil.Decidable.
+Require        riscv.Utility.InstructionNotations.
+Require Import riscv.Platform.MinimalLogging.
+Require Import bedrock2.MetricLogging.
+Require Import riscv.Platform.MetricMinimal.
+Require Import riscv.Utility.Utility.
+Require Import riscv.Utility.Encode.
+Require Import coqutil.Map.SortedList.
+Require Import compiler.StringNameGen.
+Require Import riscv.Utility.InstructionCoercions.
+Require Import riscv.Platform.MetricRiscvMachine.
+Require bedrock2.Hexdump.
+
+Open Scope Z_scope.
+Open Scope string_scope.
+Open Scope ilist_scope.
+
+Existing Instance DefaultRiscvState.
+
+Axiom TODO: forall {T: Type}, T.
+
+Instance flatToRiscvDef_params: FlatToRiscvDef.FlatToRiscvDef.parameters := {
+  funname_env T := TODO;
+  iset := RV32I;
+  FlatToRiscvDef.FlatToRiscvDef.compile_ext_call _ _ _ s :=
+    match s with
+    | FlatImp.SInteract _ fname _ =>
+      if string_dec fname "nop" then
+        [[Addi Register0 Register0 0]]
+      else
+        nil
+    | _ => []
+    end;
+}.
+
+Existing Instance coqutil.Map.SortedListString.map.
+Existing Instance coqutil.Map.SortedListString.ok.
+
+Instance pipeline_params : Pipeline.parameters. simple refine {|
+  Pipeline.string_keyed_map := _;
+  Pipeline.Registers := _;
+  Pipeline.ext_spec _ _ := TODO;
+  Pipeline.PRParams := TODO;
+|}; unshelve (try exact _); apply TODO. Defined.
+
+Instance pipeline_assumptions: @Pipeline.assumptions pipeline_params. Admitted.
+
+Definition allFuns: list Syntax.func := [
+  UnsaturatedSolinas.carry_mul;
+  UnsaturatedSolinas.carry_square;
+  UnsaturatedSolinas.carry;
+  UnsaturatedSolinas.add;
+  UnsaturatedSolinas.sub;
+  UnsaturatedSolinas.opp;
+  UnsaturatedSolinas.selectznz;
+  UnsaturatedSolinas.to_bytes;
+  UnsaturatedSolinas.from_bytes
+].
+
+Notation src_env := (SortedListString.map (list string * list string * Syntax.cmd.cmd)).
+
+Definition e: src_env := map.of_list allFuns.
+
+(* stack grows from high addreses to low addresses, first stack word will be written to
+   (stack_pastend-8), next stack word to (stack_pastend-16) etc *)
+Definition stack_pastend: Z := 2048.
+
+Definition ml: MemoryLayout := {|
+  MemoryLayout.code_start    := word.of_Z 0;
+  MemoryLayout.code_pastend  := word.of_Z (4*2^10);
+  MemoryLayout.heap_start    := word.of_Z (4*2^10);
+  MemoryLayout.heap_pastend  := word.of_Z (8*2^10);
+  MemoryLayout.stack_start   := word.of_Z (8*2^10);
+  MemoryLayout.stack_pastend := word.of_Z (16*2^10);
+|}.
+
+Unset Printing Coercions. (* https://github.com/mit-plv/fiat-crypto/issues/899 *)
+
+Definition compiled := Eval vm_compute in (compile ml e).
+
+Definition asm: list Instruction :=
+  match compiled with
+  | Some (l, _) => l
+  | None => []
+  end.
+
+Notation MapStrZ := (SortedListString.map Z).
+
+Definition positions: MapStrZ :=
+  match compiled with
+  | Some (_, e) => e
+  | None => map.empty
+  end.
+
+Definition LF : string := String (Coq.Strings.Ascii.Ascii false true false true false false false false) "".
+
+Definition ZToStr(z: Z): string := DecimalString.NilZero.string_of_int (BinInt.Z.to_int z).
+Definition natToStr(n: nat): string := ZToStr (Z.of_nat n).
+
+Fixpoint save_arg_regs(n: nat): string :=
+  match n with
+  | O => ""
+  | S m => save_arg_regs m ++ "  sw a" ++ natToStr m ++ ", " ++ ZToStr (-4 * Z.of_nat n) ++ "(sp)" ++ LF
+  end.
+
+Fixpoint load_res_regs(n: nat)(offset: Z): string :=
+  match n with
+  | O => ""
+  | S m => load_res_regs m offset ++
+           "  lw a" ++ natToStr m ++ ", " ++ ZToStr (offset + -4 * Z.of_nat n) ++ "(sp)" ++ LF
+  end.
+
+Definition call(mypos: Z)(e_src: src_env)(e_pos: MapStrZ)(f: string): (string * Z) :=
+  match map.get e_src f, map.get e_pos f with
+  | Some (argvars, resvars, body), Some funpos => (
+  "  addi sp, sp, -4" ++ LF ++
+  "  sw ra, 0(sp)" ++ LF ++
+  save_arg_regs (List.length argvars) ++
+  "  jal ra, " ++ ZToStr (funpos - (mypos + 4 * (2 + Z.of_nat (List.length argvars)))) ++ LF ++
+  load_res_regs (List.length resvars) (- Z.of_nat (List.length argvars)) ++
+  "  lw ra, 0(sp)" ++ LF ++
+  "  addi sp, sp, 4" ++ LF ++
+  "  ret" ++ LF,
+  4 * (Z.of_nat (2 + List.length argvars + 1 + List.length resvars + 3)))
+  | _, _ => ("ERROR: " ++ f ++ " not found", -1)
+  end.
+
+Fixpoint wrappers(mypos: Z)(e_src: src_env)(e_pos: MapStrZ)(fs: list string): string :=
+  match fs with
+  | f :: rest => let '(s, l) := call mypos e_src e_pos f in
+                 ".globl " ++ f ++ LF ++
+                 f ++ ":" ++ LF ++
+                 s ++
+                 wrappers (mypos + l) e_src e_pos rest
+  | nil => ""
+  end.
+
+Definition asm_str: string :=
+  Eval vm_compute in
+  ".section .text" ++ LF ++
+  "bedrock2functions: .incbin ""poly1305.bin""" ++ LF ++
+  wrappers (4 * (Z.of_nat (List.length asm))) e positions (map.keys positions).
+
+From bedrock2 Require Import ToCString Bytedump.
+Local Open Scope bytedump_scope.
+Goal True.
+  let c_code := eval vm_compute in (byte_list_of_string asm_str) in idtac c_code.
+Abort.
